
#statistics #uoft/sta237 

For any events A and C, If *P(A) > 0* and *P(C) > 0* then  
$$P(A\cap C) = P(A|C)P(C) = P(C|A)P(A)$$

---


# Derivation
Derived from the definition of [Conditional Probability](Conditional%20Probability.md)  
The **Conditional Probability** of **A given C** given A and C is  
$$P(A|C) \ = \ \frac{P(A\cap C)}{P(C)}$$  
The Multiplication Rule is rewritten by  
$$P(A\cap C) =P(A|C)P(A)$$

# Uses
Can be helpful by decomposing computing the probability of $A\cup C$  
Can be rewritten to become [Bayes Rule](Bayes%20Rule.md)